implementation in progress

transitive_closure.v
@@ -7,976 +7,227 @@ Set Implicit Arguments.
 
 
 
+Section AllButLast.
+
+  Variable X: Type.
+  
+  Definition belast (xs: seq X) :=
+    (fix belast xs := 
+    match xs with
+      | [::] => [::]
+      | [::x] => [::]
+      | x::xs => x::(belast xs)
+    end)
+    xs.
+
+  Definition allbutlast p xs :=
+    all p (belast xs).
+
+  Lemma allbutlast_impl (p q: pred X) xs:
+    (forall x, p x -> q x) ->
+    allbutlast p xs ->
+    allbutlast q xs.
+  Proof.
+    elim: xs => [|x xs IHxs].
+      by [].
+    case: xs IHxs => [|y xs IHxs].
+      by [].
+    rewrite /allbutlast /=.
+    move => H0 /andP [] /H0 -> /=.
+    by move: (IHxs H0). 
+  Qed.
+
+  Lemma allbutlast_cons (p: pred X) x xs: p x -> allbutlast p xs -> allbutlast p (x::xs).
+  Proof.
+    elim: xs x => [|y xs IHxs] x //. 
+    by rewrite /allbutlast /= => -> /=.
+  Qed.
+
+  Lemma allbutlast_cons' p x y xs: allbutlast p (x::y::xs) -> p x && allbutlast p (y::xs).
+  Proof.
+    elim: xs x => [|z xs IHxs] x //. 
+  Qed.
+  
+  Lemma all_allbutlast p xs: all p xs -> allbutlast p xs.
+  Proof.
+    elim: xs => [|x xs IHxs] //.
+    move => /= /andP [] H0 /IHxs.
+    by apply: allbutlast_cons.
+  Qed.
+       
+  Lemma all_allbutlast_cat p xs ys: all p xs -> allbutlast p ys -> allbutlast p (xs++ys).
+  Proof.
+    elim: xs => [|x xs IHxs].
+      by rewrite /= => _.
+    rewrite /= => /andP [] H0. 
+    move => H1 H2. move: (IHxs H1 H2).
+    by apply: allbutlast_cons.
+  Qed.
+
+  Lemma allbutlast_last p x xs: allbutlast p xs -> p (last x xs) -> all p xs.
+  Proof.
+    elim: xs x => [|y xs IHxs] x //.
+    case: xs IHxs => [|z xs] IHxs.
+      by rewrite /allbutlast /= => -> ->.
+    move/allbutlast_cons'/andP => [] H0 H1 H2.
+    move: (IHxs x H1 H2).
+    by rewrite /= H0 => /andP [] ->.
+  Qed.
+                         
+End AllButLast.   
+
+
 Section TransitiveClosure.
 
-Variable char: finType.
-Variable A: nfa char.
-
-
-
-Lemma mem_der_Plus r s w : w \in (@Plus char r s) = (w \in r) || (w \in s).
-Proof. elim: w r s => [|a w IHw] r s //=. Qed.
-
-Lemma der_Plus a r s : der a (@Plus char r s) = Plus (der a r) (der a s).
-Proof. by []. Qed.
-
-Lemma mem_der_Conc r s (w1 w2: word char) : w1 \in r ->  w2 \in s ->
- (w1 ++ w2) \in (Conc r s).
-Proof.
-  move => H0 H1.
-  apply/concP.
-  exists w1.
-    by rewrite H0.
-  exists w2.
-    by rewrite H1.
-  reflexivity.  
-Qed.
-
-
-Lemma der_fold_Plus (r: regular_expression char) rs (a: char): der a (foldr (@Plus char) r rs) = foldr (@Plus char) (der a r) (map (der a) rs).
-Proof.
-elim: rs r a => [|s rs IHrs] r a //=.
-by rewrite IHrs.
-Qed.
-
-Lemma mem_der_fold_Plus (r: regular_expression char) rs w: (w \in r) || has (fun r => w \in r) rs = (w \in (foldr (@Plus char) r rs)).
-Proof.
-  elim: rs r w => [|s rs IHrs] r w.
-    apply/orP/idP.
-      move => [] //=.
-    by firstorder.
-  rewrite /= mem_derE mem_derE mem_derE mem_der_Plus.
-  apply/orP/idP.
-  move => [] H0; apply/orP.
-      right. rewrite -mem_derE -IHrs. by rewrite H0.
-    apply/orP. move/orP: H0 => [].
-      by move => ->.
-    rewrite -IHrs => ->.
-    apply/or3P. by firstorder.
-  move/orP => [].
-    move => ->. by firstorder.
-  rewrite -IHrs. move/orP => [].
-    by firstorder.
-  move => ->. right. by rewrite orbT.
-Qed.
+  Variable char: finType.
+  Variable A: dfa char.
   
-Lemma has_eps_fold_Plus r rs: has_eps r || has (@has_eps _) rs = has_eps (foldr (@Plus char) r rs).
-Proof.
-  elim: rs r => [|s rs IHrs] r.
-    by rewrite orbF.
-  simpl. rewrite -(IHrs r).
-  by rewrite orbCA.
-Qed.
+    Section Misc.
+      Lemma Plus_dist r s (w: word char): w \in Plus r s = (w \in r) || (w \in s). 
+      Proof. by rewrite -topredE. Qed.
+      Lemma foldr_Plus r rs (w: word char):
+        w \in foldr (@Plus char) r rs = (w \in r) || has (fun r => w \in r) rs. 
+      Proof.
+        elim: rs r => [|s rs IHrs] r /=. 
+          by rewrite orbF.
+        rewrite orbCA -IHrs.
+        by rewrite -topredE -topredE.
+      Qed.
+    End Misc.
 
-Lemma mem_der_Void w: mem_der (@Void char) w = false.
-Proof. elim: w => [|a w IHw] //=. Qed.
+  Lemma minn_to_ord m n: minn m n <= n.
+  Proof. elim: n m => [|n IHn] m /=.
+    by rewrite /minn.
+    rewrite /minn.
+    case_eq (m < n.+1).
+    by apply: ltnW.
+    move => _. by apply: ltnSn.
+  Qed.
 
-Lemma mem_der_Eps w: mem_der (@Eps char) w -> w = [::].
-Proof. elim: w => [|a w IHw] //=. by rewrite mem_der_Void. Qed.
+  Lemma leq_ltn_gt0 n m: m > 0 -> n <= m.-1 -> n < m.
+  Proof.  elim: m n => [|m IHm] n //=. Qed.
 
-Lemma mem_der_Atom a w: mem_der (@Atom char a) w -> w = [::a].
-Proof. elim: w a => [|b w IHw] a //=. case_eq (b==a).
-  by move/eqP => -> /mem_der_Eps ->.
-by rewrite mem_der_Void.
-Qed.
+  Lemma A_has_states: #|A| > 0.
+  apply/card_gt0P.
+  by exists (dfa_s0 A).
+  Qed.
+  
+  (* this represents k in 'I_#|A| *)
+  Definition k1_ord k := 
+    Ordinal (leq_ltn_gt0 _ _ A_has_states (minn_to_ord k #|A|.-1)).
 
-Lemma cons_eq a b (w1 w2: word char):
-  a::w1 = b::w2 -> a=b /\ w1 = w2.
-Proof.
-  move => H0.
-  move: (f_equal (head a) H0) => /=.
-  by move: (f_equal behead H0) => /=.                                   
-Qed.
-                                    
-Lemma mem_der_Conc3 r s w:
-(exists w1, exists w2, w1 ++ w2 = w /\ mem_der r w1 /\ mem_der s w2) -> mem_der (@Conc char r s) w.
-Proof.
-  elim: w r s => [|a w IHw] r s /=.
-    move => [] w1 [] w2 [].
-    case: w1 => [] //. case: w2 => [] //=.
-    by move => _ [] -> ->.
-  move => [] w1 [] w2 [].
-  case_eq (has_eps r) => H0.
-    rewrite mem_der_Plus.
-    case: w1 => [|b w1].
-      move => /= -> [] _ /= ->.
-      by rewrite orbT.
-    rewrite cat_cons.
-    move/cons_eq => [] -> <- [] H1 H2.
-    by rewrite mem_der_Conc.
-  case: w1 => [|b w1].
-    move => _ [] /=. by rewrite H0. 
-  rewrite cat_cons.
-  move/cons_eq => [] -> <- [] H1 H2.
-  by rewrite mem_der_Conc.  
-Qed.
+  Lemma k1_ord_lt k: k1_ord k < k.+1.
+  Proof.
+    rewrite /k1_ord /=.
+    case_eq (k <= #|A|.-1) => H0.
+      rewrite minnl => //.
+    move: (leq_total k #|A|.-1).
+    rewrite H0 /= => H1.
+    by rewrite minnr.
+  Qed.
+    
+  Fixpoint R (k: nat) (i j: 'I_#|A|) : regular_expression char :=
+    match k with
+      |   0  => 
+            let r := foldr (@Plus _) (Void _) (map (@Atom _) (filter [pred a | dfa_step A (enum_val i) a == (enum_val j)] (enum char))) in
+              if i == j then Plus r (Eps _) else r
+      | k.+1 =>
+          let k' := k1_ord k in
+            Plus (
+                Conc (R k i k')
+                     (Conc (Star (R k k' k')) (R k k' j))
+              )
+                 (R k i j)
+    end.        
+
+  Notation "'R^' k" := (R k) (at level 8).
+
+  
+  Definition L (k: nat) (x y: A) : pred (word char) :=
+    [pred w | 
+    (last x (dfa_run' A x w) == y)
+         && allbutlast (fun x => enum_rank x < k) (dfa_run' A x w) 
+    ].
+  Notation "'L^' k" := (L k) (at level 8).
 
 
-Lemma mem_der_Conc2 r s w: mem_der (@Conc char r s) w -> exists w1, exists w2, w1 ++ w2 = w /\ mem_der r w1 /\ mem_der s w2.
-Proof.
-  elim: w r s => [|a w IHw] r s /=.
-    move => /andP [H0 H1].
-    exists [::]. by exists [::].
-  case_eq (has_eps r) => H0.
-    rewrite mem_der_Plus => /orP [].
-      move/IHw => [] w1 [] w2 [] <- [] H1 H2.
-      exists (a::w1). exists w2.
-      split.
+  Section L.
+    Lemma L_monotone k i j w: w \in L^k i j -> w \in L^(k.+1) i j.
+    Proof.
+      rewrite -2!topredE /= /L /= => /andP [] -> /=.
+      apply: allbutlast_impl.
+      move => x.
+      by apply: (@ltnW ((enum_rank x)) k).
+    Qed.
+
+    Lemma L_catL k i j w1 w2:
+      w1 \in L^k i (enum_val (k1_ord k)) ->
+      w2 \in L^k.+1 (enum_val (k1_ord k)) j ->
+      w1++w2 \in L^k.+1 i j.
+    Proof.
+      rewrite /L -3!topredE /=.
+      rewrite dfa_run'_cat.
+      move => /andP [] /eqP H0 H1 /andP [] /eqP H2 H3.
+      case: w1 H0 H1 => [|v1 w1] H0 H1.
+        rewrite /= in H0.
+        rewrite H0 /= H2 eq_refl /=.  
+        exact: H3.
+      rewrite last_cat.
+      case: w2 H2 H3 => [|v2 w2] H2 H3.
+        rewrite /= in H2.
+        rewrite -H2 H0 /= eq_refl /=.
+        eapply allbutlast_impl.
+        move => x. by eapply (@ltnW ((enum_rank x)) k).
+        rewrite cats0.
+        exact H1.
+
+      rewrite H0 H2 eq_refl andTb.
+      eapply all_allbutlast_cat.
+        apply: (allbutlast_last _ i) => //. 
+          eapply allbutlast_impl.
+          move => x.
+          by eapply (@ltnW ((enum_rank x)) k).
         by [].
-      by rewrite /= H1 H2.
-    move => H1.
-    exists [::]. exists (a::w).
-    split.
+        rewrite H0. 
+        rewrite enum_valK.
+        by apply: k1_ord_lt.
       by [].
-    by rewrite /= H0 H1.
-  move/IHw => [] w1 [] w2 [] <- [] H1 H2.
-  exists (a::w1). exists w2.
-  split.
-    by [].
-  by rewrite /= H1 H2.
-Qed.
+      Qed.
 
-Lemma mem_der_Star r w: mem_der (@Star char r) w -> w = [::] \/ mem_der (Conc r (Star r)) w.
-Proof.
-  elim: w r => [|a w IHw] r /=.
-    by firstorder.
-  move/mem_der_Conc2 => [] w1 [] w2 [] H0 [] H1 H2.
-  right.
-  rewrite -H0.
-  case_eq (has_eps r) => H3.
-    rewrite mem_der_Plus.
-    apply/orP. left.
-    by rewrite mem_der_Conc.
-  by rewrite mem_der_Conc.
-Qed.
-  
-Lemma minn_to_ord m n: minn m n <= n.
-Proof. elim: n m => [|n IHn] m /=.
-  by rewrite /minn.
-rewrite /minn.
-case_eq (m < n.+1).
-  by apply: ltnW.
-move => _. by apply: ltnSn.
-Qed.
-
-Lemma noname n m: m > 0 -> n <= m.-1 -> n < m.
-Proof.  elim: m n => [|m IHm] n //=. Qed.
-
-Lemma A_has_states: #|A| > 0.
-apply/card_gt0P.
-by exists (nfa_s0 A).
-Qed.
-  
-(* this represents k in 'I_#|A| *)
-Definition k1_ord k := 
-  Ordinal (noname _ _ A_has_states (minn_to_ord k #|A|.-1)).
-  
-Fixpoint R (k: nat) (i j: 'I_#|A|) : regular_expression char :=
-match k with
-|   0  => 
-      let r := foldr (@Plus _) (Void _) (map (@Atom _) (filter [pred a | nfa_step A (enum_val i) a (enum_val j)] (enum char))) in
-      if i == j then Plus r (Eps _) else r
-| k.+1 =>
-    let k' := k1_ord k in
-    Plus (
-        Conc (R k i k')
-             (Conc (Star (R k k' k')) (R k k' j))
-        )
-        (R k i j)
-end.        
-
-Definition nfa_R (k: nat) (i j: 'I_#|A|) : nfa char :=
-nfaI
-  char
-  (option_finType A)
-  (Some (enum_val i))
-  [pred x | if x is Some x then i == j else true ]
-  (fun x a y =>
-     match x with
-         | None => false
-         | Some x =>
-         match y with
-             | None => nfa_step A x a (enum_val j) && ((enum_rank x == i) || (enum_rank x < k))
-             | Some y => nfa_step A x a y && (enum_rank y < k) && ((enum_rank x == i) || (enum_rank x < k))
-         end
-  end).
-
-Lemma nfa_R_correct2_0 w i j: mem_der (R 0 i j) w -> nfa_accept (nfa_R 0 i j) (Some (enum_val i)) w.
-Proof.
-  elim: w i j => [|a w IHw] i j.
-    simpl.
-    case_eq (i==j).
-      by move/eqP => ->.
-    move => H0. rewrite H0.
-    rewrite -has_eps_fold_Plus. 
-    rewrite orFb.
-    move/hasP => [] r.
-    by move/mapP => [] a _ ->.
-  case_eq (i==j) => /=.
-    move/eqP => ->. rewrite eq_refl /=.
-    rewrite der_fold_Plus mem_der_Plus.
-    rewrite -mem_der_fold_Plus.
-    rewrite mem_der_Void.
-    rewrite orbF orFb.
-    move/hasP => [] r /mapP [] s /mapP [] c.
-    rewrite mem_filter /= => /andP [] H0 _.
-    move => -> -> /=.
-    case_eq (a==c) => /=.
-      move/eqP => ->.
-      move/mem_der_Eps => H1.
-      rewrite H1. rewrite H1 in IHw.
-      apply/existsP. exists (None).
-      by rewrite enum_valK eq_refl H0 /=.
-    by rewrite mem_der_Void.  
-  move => H0. rewrite H0.  
-  rewrite der_fold_Plus -mem_der_fold_Plus mem_der_Void orFb.
-  move/hasP => [] r /mapP [] s /mapP [] c.
-  rewrite mem_filter => /= /andP [] H1 _.
-  move => -> -> /=.
-  case_eq (a==c) => /=.
-    move/eqP => ->. move/mem_der_Eps => ->.
-    apply/existsP. exists (None).
-    by rewrite enum_valK eq_refl /= H1.
-  by rewrite mem_der_Void.  
-Qed.
-
-Lemma nfa_R_monotone k w i j x: nfa_accept (nfa_R k i j) x w -> nfa_accept(nfa_R k.+1 i j) x w.
-Proof.
-  elim: w k i j x => [|a w IHw] k i j [x|] //;
-  move => /= /pred0Pn;
-  move => [] [y|] /andP [] //.
-    move => /andP [] /andP [] H0 H1 /orP [] H2 H3;
-    apply/pred0Pn; exists (Some y).
-          rewrite H0 (leqW H1) H2 /=.
-          by apply: IHw.
-        rewrite H0 (leqW H1) (leqW H2) orbT /=.
-        by apply: IHw.
-      move => /andP [] H0 /orP [] H1 H2;
-      apply/pred0Pn; exists (None).
-      rewrite H0 H1 /=.
-      by apply: IHw.
-    rewrite H0 (leqW H1) 1!orbT /=.
-    by apply: IHw.
-Qed.
-
-Lemma enum_rank_ltn (x: A): enum_rank x <= #|A|.-1.
-Proof.
-  rewrite -(leq_add2r 1) 2!addn1.
-  rewrite (prednK A_has_states).
-  exact: (ltn_ord (enum_rank x)) => /=.
-Qed.  
-
-Lemma k1_ord_leq_k k: nat_of_ord (k1_ord k) <= k.
-Proof.
-  rewrite /k1_ord.
-  case_eq (k <= #|A|.-1) => H0 /=.
-    by rewrite (minnl H0).
-  move: (leq_total k #|A|.-1).
-  rewrite H0 orFb => H1.
-  by rewrite (minnr H1).
-Qed.
-  
-Lemma nfa_R_lpath_start k i j x xs a w:
-  nfa_lpath (nfa_R k i j) (Some x) xs (a::w) ->
-  (enum_rank x == i) || (enum_rank x < k).
-Proof.
-  elim: xs => [|[y|] xs IHxs] //;
-  move => /= /andP [] /andP [].
-    by [].
-  by [].
-Qed.          
-
-Lemma nfa_R_lpath_empty k i j x xs:
-  nfa_lpath (nfa_R k i (k1_ord k)) x xs [::] ->
-  nfa_lpath (nfa_R k i j) x xs [::].
-Proof.
-  elim: xs x => [|y xs IHxs] x //=.
-Qed.  
-
-Lemma nfa_R_lpath_empty2 k i j x xs:
-  nfa_lpath (nfa_R k i j) x xs [::] ->
-  nfa_lpath (nfa_R k i (k1_ord k)) x xs [::].
-Proof.
-  elim: xs x => [|y xs IHxs] x //=.
-Qed.  
-
-Lemma nfa_R_correct2' k i j x xs w : 
-  nfa_lpath (nfa_R k i (k1_ord k)) x xs w ->
-  nfa_lpath (nfa_R k.+1 i j) x xs w.
-Proof.
-  elim: w k i j x xs => [|a w IHw] k i j x xs; elim: xs => [|y xs _]  //.
-  move => /= /andP [] /andP [] /andP [] H0 /orP [] H2 /orP [] H3 H4;
-  rewrite H0 2!ltnS.
-        rewrite H2 (eqP H3) (k1_ord_leq_k) orbT /=.
-        by apply: IHw.
-      rewrite H2 (ltnW H3) orbT /=.
-      by apply: IHw.
-    rewrite (ltnW H2).
-    move/eqP: H3 => /(@f_equal 'I_#|A| nat (@nat_of_ord #|A|)) /eq_leq H3.
-    rewrite (leq_trans H3 (k1_ord_leq_k k)) 2!orbT /=.
-    by apply: IHw.
-  rewrite (ltnW H2) (ltnW H3) 2!orbT /=.
-  by apply: IHw.
-Qed.        
-
-Lemma nfa_R_correct2'' k i j x xs w : 
-  nfa_lpath (nfa_R k (k1_ord k) j) x xs w ->
-  nfa_lpath (nfa_R k.+1 i j) x xs w.
-Proof.
-  elim: w k i j x xs => [|a w IHw] k i j x xs; elim: xs => [|y xs _]  //.
-  move => /= /andP [] /andP [] /andP [] H0 /orP [] H2 /orP [] H3 H4;
-  rewrite H0 2!ltnS.
-        move/eqP: H2 => /(@f_equal 'I_#|A| nat (@nat_of_ord #|A|)) /eq_leq H5.
-        rewrite H3 (leq_trans H5 (k1_ord_leq_k k)) orbT /=.
-        by apply: IHw.
-      move/eqP: H2 => /(@f_equal 'I_#|A| nat (@nat_of_ord #|A|)) /eq_leq H5.
-      rewrite (ltnW H3) (leq_trans H5 (k1_ord_leq_k k)) 2!orbT /=.
-      by apply: IHw.
-    rewrite (ltnW H2) H3 orbT /=.
-    by apply: IHw.
-  rewrite (ltnW H2) (ltnW H3) 2!orbT /=.
-  by apply: IHw.
-Qed.
-
-Lemma nfa_R_correct2''' k i j x xs w : 
-  nfa_lpath (nfa_R k (k1_ord k) (k1_ord k)) x xs w ->
-  nfa_lpath (nfa_R k.+1 i j) x xs w.
-Proof.
-  elim: w k i j x xs => [|a w IHw] k i j x xs; elim: xs => [|y xs _]  //.
-  move => /= /andP [] /andP [] /andP [] H0 /orP [] H2 /orP [] H3 H4;
-  rewrite H0 2!ltnS.
-        move/eqP: H2 => /(@f_equal 'I_#|A| nat (@nat_of_ord #|A|)) /eq_leq H5.
-        rewrite (leq_trans H5 (k1_ord_leq_k k)) orbT /=.
-        move/eqP: H3 => /(@f_equal 'I_#|A| nat (@nat_of_ord #|A|)) /eq_leq H6.
-        rewrite (leq_trans H6 (k1_ord_leq_k k)) orbT /=.
-        by apply: IHw.
-      move/eqP: H2 => /(@f_equal 'I_#|A| nat (@nat_of_ord #|A|)) /eq_leq H5.
-      rewrite (ltnW H3) (leq_trans H5 (k1_ord_leq_k k)) 2!orbT /=.
-      by apply: IHw.
-    rewrite (ltnW H2) orbT /=.
-    move/eqP: H3 => /(@f_equal 'I_#|A| nat (@nat_of_ord #|A|)) /eq_leq H6.
-    rewrite (leq_trans H6 (k1_ord_leq_k k)) orbT /=.
-    by apply: IHw.
-  rewrite (ltnW H2) (ltnW H3) 2!orbT /=.
-  by apply: IHw.
-Qed.
-
-(*
-Lemma mem_der_Star_ind (p: word char -> Prop) r:
-  p [::] ->
-  (forall w1 w2, mem_der r w1 -> mem_der (Star r) w2 -> p w2 -> p (w1 ++ w2)) ->
-  forall (w: word char), mem_der (Star r) w -> p w.
-Proof.
-  move => H0 H1 w.
-  move/mem_der_Star => [].
-    by move => ->.
-  move/mem_der_Conc2 => [] w1 [] w2 [] <- [].
-  move => H2 H3.
-  apply: H1 => //.
-          
-    
-  elim: w2 w1 => [|a w2 IHw2] w1.
-    move => H2 H3.
-    by apply: H1.
-  move => H2 H3.
-  move: (mem_der_Conc _ _ w1 (a::w2) H2 H3).    
-  rewrite -cat_rcons.
-  move/mem_der_Conc2 => [] w3 [] w4 [] .
-  apply: IHw2.
-*)
-
-(*
-Lemma nfa_R_correct2_Star k i j w1 w2:
-  (forall (w : word char) (i j : 'I_#|A|),
-        mem_der (R k i j) w -> nfa_accept (nfa_R k i j) (enum_val i) w) ->
-  mem_der (Star (R k (k1_ord k) (k1_ord k))) (w1 ++ w2) -> exists xs, nfa_lpath (nfa_R k.+1 i j) (enum_val (k1_ord k)) xs (w1 ++ w2) /\ last (enum_val (k1_ord k)) xs = enum_val (k1_ord k).
-Proof.
-  move => H0.
-
-  elim: w1 w2 i j k H0 => [|a w1 IHw1] w2 i j k H0.
-  
-  
-  elim: w i j => [|a w IHw] i j.
-    move => _. by exists [::].
-  simpl.
-  
-  move/mem_der_Conc2 => [] w1 [] w2 [] H1 [].
-  rewrite -H1 in IHw. rewrite -H1.
-  move => H2.
-    assert (mem_der (R k (k1_ord k) (k1_ord k)) (a::w1)) => //.
-  
-  elim: w2 w1 H1 IHw H2 H => [|b w2 IHw2] w1 H1 IHw H2 H.
-    move => _.
-    move/nfa_accept_lpath: (H0 _ _ _ H) => [] xs [].
-    move/(nfa_R_correct2''' _ i j) => H3.
-    move/eqP => H4.
-    rewrite cats0. 
-    by exists xs.
-
-  move => /= /mem_der_Conc2 [] w3 [] w4 [] H3 [].
-    
-Admitted.
-*)
-
-Lemma R_monotone k i j w: mem_der (R k i j) w -> mem_der (R k.+1 i j) w.
-Proof. rewrite /= mem_der_Plus => ->. by rewrite orbT. Qed.
-
-Check seq_ind.
-
-Lemma cat_ind (P: word char -> Prop):
-  P [::] ->
-  (forall w1 w2, P w2 -> P (w1 ++ w2)) ->
-  forall w, P w.
-Proof.
-  move => H0 H1 w.
-  elim: w => [|a w IHw] //.
-  rewrite -cat1s.
-  by apply: H1.
-Qed.
-
-
-Lemma R0_cons i j a w:
-  mem_der (R 0 i j) (a::w) ->
-  w = [::] /\ nfa_step (nfa_R 0 i j) (enum_val i) a (enum_val j).
-Proof.
-  move => /=.
-  rewrite fun_if der_Plus der_fold_Plus -map_comp.
-  rewrite fun_if if_arg mem_der_Plus -mem_der_fold_Plus mem_der_Void orFb.
-  rewrite 2!enum_valK 2!eq_refl /= 2!andbT.
-  case_eq (i == j) => H1; rewrite H1.
-    move/orP => [] //.
-    move/hasP => [] r /mapP [] b. rewrite mem_filter => /andP [] /=.
-    case_eq (a == b).
-      by move/eqP => -> -> _ -> /mem_der_Eps ->.
-    move => _ _ _ ->.
-    by rewrite mem_der_Void.
-  move/hasP => [] r /mapP [] b. rewrite mem_filter => /andP [] /=.
-  case_eq (a == b).
-    by move/eqP => -> -> _ -> /mem_der_Eps ->.
-  move => _ _ _ ->.
-  by rewrite mem_der_Void.
-Qed.  
-  
-Lemma R0_nil i j:
-  mem_der (R 0 i j) [::] =
-  (j == i).
-Proof.
-  rewrite /= fun_if -has_eps_fold_Plus /= orbT.
-  case_eq (i == j) => H0; rewrite H0.
-    by rewrite eq_sym H0.
-  apply/hasP/idP.
-    by move => /= [] r /mapP [] a _ ->.
-  by rewrite eq_sym H0.
-Qed.
-                     
-Lemma R_der_step k i j a w m:
-  mem_der (R k i j) (a::w) ->
-  nfa_step (nfa_R k i j) (enum_val i) a (enum_val m) ->
-  mem_der (R k m j) w.
-Proof.
-  elim: k w i j a m => [|k IHk] w i j a m H0.
-    move: (R0_cons _ _ _ _ H0) => [] H1 H2.
-    rewrite H1. rewrite H1 in H0.
-    move => /andP [] /andP [] H3 /orP [] H4 /orP [] H5 //.
-    rewrite enum_valK in H5.
-    by rewrite R0_nil eq_sym H5.
-  move: H0. rewrite /= mem_der_Plus.
-  move/orP => [].
-    case_eq (has_eps (R k i (k1_ord k))) => H0.
-    rewrite mem_der_Plus => /orP [].
-    move/mem_der_Conc2 => [] w1 [] w2 [] <-.
-    
-    move => /andP [] /andP [] H3 /orP [] H4 /orP [] H5 //.
-           rewrite enum_valk
-           
-    
-      
-
-Lemma R_der k i j a w:
-  mem_der (der a (R k i j)) w ->
-  mem_der (R k j j) w \/ 
-  exists m: 'I_#|A|,
-    m < k /\
-    mem_der (R k i m) [::a] /\
-    mem_der (R k m j) w.
-Proof.
-  elim: k i j a w => [|k IHk] i j a w.
-    move => /=.
-    rewrite eq_refl.
-    rewrite fun_if der_Plus der_fold_Plus.
-    case_eq (i==j) => H0; rewrite H0.
-      move/eqP: H0 => ->.
-      rewrite mem_der_Plus => /orP [].
-        rewrite -mem_der_fold_Plus => /orP [].
-          by rewrite mem_der_Void.
-        move/hasP => [] r /mapP [] s /mapP [] b.
-        rewrite mem_filter => /andP [].
-        move => H0 _ -> -> /=.
-        case_eq (a == b).
-          move => _ /mem_der_Eps -> /=.
-          left. by rewrite orbT.
-        by rewrite mem_der_Void.
-      by rewrite /= mem_der_Void.
-    rewrite -mem_der_fold_Plus.
-    move/orP => [].
-      by rewrite mem_der_Void.
-    move/hasP => [] r /mapP [] s /mapP [] b.
-    rewrite mem_filter => /andP [].
-    move => H1 _ -> -> /=.
-    case_eq (a == b).
-      move => _ /mem_der_Eps -> /=.
-      left. by rewrite orbT.
-    by rewrite mem_der_Void.
-  rewrite /= mem_der_Plus => /orP [].
-    case_eq (has_eps (R k i (k1_ord k))) => H0.
-      rewrite mem_der_Plus => /orP [].
-        right.
-        exists (k1_ord k).
-        split.
-          by apply: k1_ord_leq_k.
-        split.
-          
-      
-      
-
-Lemma nfa_R_correct_Star k w:
-  mem_der (Star (R k (k1_ord k) (k1_ord k))) w ->
-  w = [::] \/ mem_der (R k.+1 (k1_ord k) (k1_ord k)) w.
-Proof.
-  (*move: w k. apply: cat_ind => [|w1 w2 IHw] k.*)
-  elim: w k => [|a w IHw] k.
-  
-    move/mem_der_Star => [].
-      by firstorder.
-    move/mem_der_Conc2 => [] w1 [] w2 [].
-    case: w1 => [] //. case: w2 => [] //.
-    by firstorder.
-  rewrite 1!/= => H0.
-  rewrite mem_der_Plus.
-  right.
-  apply/orP.
-  case_eq (has_eps (R k (k1_ord k) (k1_ord k))) => H1.
-    left.
-    rewrite mem_der_Plus.
-    apply/orP. left.
-    apply: mem_der_Conc3.
-    move/mem_der_Conc2: H0 => [] w1 [] w2 [] <- [] H2 H3.
-    exists w1. exists w2.
-    firstorder.
-    apply: mem_der_Conc3.
-    exists w2. exists [::].
-    firstorder.
-    by rewrite cats0.
-  move/mem_der_Conc2: H0 => [] w1 [] w2 [] H2 [] H3 H4.
-  rewrite -H2.
-  elim: w2 w1 H3 H2 H4 => [|b w2 IHw2] w1 H3 H2 H4.
-    right. by rewrite cats0.
-  move/mem_der_Star: H4 => [] //=.
-  rewrite H1 => /mem_der_Conc2 [] w3 [] w4 [] H4 [] H5 H6.
-  
-  
-  left.
-  apply: mem_der_Conc => //=.
-   
-    
-  
-Lemma nfa_R_correct2 k w i j: mem_der (R k i j) w -> nfa_accept (nfa_R k i j) (enum_val i) w.
-Proof.
-  elim: k w i j => [|k IHk] w i j.
-    exact: nfa_R_correct2_0.
-  simpl.
-  rewrite mem_der_Plus.
-  move/orP => [].
-    move/mem_der_Conc2 => [] w1 [] w2 [] H0 [] /IHk /nfa_accept_lpath [] xs1 [] H1 H2.
-    rewrite -H0. clear H0.
-    move/mem_der_Conc2 => [] w3 [] w4 [] H3 [] H4 /IHk /nfa_accept_lpath [] xs2 [] H5 H6.
-    rewrite -H3. clear H3.
-    apply/nfa_accept_cat.
-    exists xs1.
-    move/eqP: H2 => /= ->.
-    move: H1 => /(nfa_R_correct2' _ _ j) => -> /=.
-    
-    apply/nfa_accept_cat.
-    exists xs2.
-    apply/andP. split.
-      clear H5 H6
-    
-    
-    move: (mem_der_Star _ _ H4) => [].
-      move => H7. rewrite H7.
-      apply: nfa_lpath_accept.
-        eapply nfa_R_correct2''.
-        eassumption.
-      exact: H6.
-    move/mem_der_Conc2 => [] w5 [] w6 [] H7 [] /IHk H8 _.
-
-    apply: mem_der
-        
-        
-      
-    
-    exists xs2.
-      move => ->. case: xs2 H5 H6 => [|x xs2] H5 H6.
-      simpl.
-          
-      
-    
-
-  case: w IHw => [|b w] IHw.
-    rewrite orFb orbF.
-    move/hasP => [] r /mapP [] s /mapP [] c.
-    rewrite mem_filter /= => /andP [] H0.
-    move => _ -> -> /=.
-    case_eq (a==c) => [/eqP ->|] //= _.
-    apply/existsP. exists (enum_val j).
-    by rewrite enum_valK 2!eq_refl H0.
-       
+  End L.
             
-     
-Lemma nfa_R_correct2 k i j w : mem_der (R k i j) w -> nfa_fin A (enum_val j) -> nfa_accept (nfa_R k i j) (enum_val i) w.
-Proof.
-  elim: k w i j => [|k IHk] w i j.
-    case_eq (i == j).
-      move/eqP => ->.
-      rewrite /= eq_refl.
-      rewrite mem_der_Plus -mem_der_fold_Plus.
-      move/orP => [].
-        move/orP => [].
-        elim: w => [|a w IHw] //=.
+  
+
+  Lemma R_L k i j w: w \in R^k i j -> w \in L^k (enum_val i) (enum_val j).
+   Proof.
+    elim: k i j w => [|k IHk] i j w.
+      case_eq (i==j) => H0 /=.
+        rewrite H0 /=.
+        rewrite Plus_dist => /orP [].
+          rewrite foldr_Plus => /orP [] //.
+          move/hasP => [] r /mapP [] a.
+          rewrite mem_filter /= => /andP [] H1 _ ->.
+          rewrite -topredE /= /atom /= => /eqP ->.
+          by rewrite -topredE /= /L /= H1.
+        rewrite -topredE /= /eps /= => /eqP ->.
+        move/eqP: H0 => ->.
+        by rewrite -topredE /= /L /= eq_refl.
+      rewrite H0.
+      rewrite foldr_Plus => /orP [] //.
+      move/hasP => [] r /mapP [] a.
+      rewrite mem_filter /= => /andP [] H1 _ ->.
+      rewrite -topredE /= /atom /= => /eqP ->.
+      by rewrite -topredE /= /L /= H1.
+
+    rewrite /= Plus_dist => /orP [].
+      rewrite -topredE /= => /concP [] w1 /IHk H1 [] w23.
+      move => /concP [] w2 H2 [] w3 /IHk H3.
+      move => Eq1 Eq2.
+      move/starP: H2 => [] vv Hvv Eqvv.
+      pose k' := enum_val (k1_ord k). 
+      assert ((flatten vv) \in L^(k.+1) k' k').
+        elim: vv w2 Eq1 Eqvv Hvv => [|v vv IHvv] w2 Eq1 Eqvv Hvv.
+          by rewrite /= -topredE /= /L /= eq_refl.
         
       
-
-Lemma nfa_R_correct k (i j: 'I_#|A|) w: nfa_fin A (enum_val j) -> nfa_accept (nfa_R k i j) (enum_val i) w -> mem_der (R k i j) w.
-Proof.
-
-  elim: k w i j => [|k IHk] w i j.
-    elim: w i j => [|a w IHw] i j.
-      case_eq (i==j).
-        move/eqP => -> H0 _ /=.
-        by rewrite eq_refl /= orbT.
-      move => H1 H0 /eqP /(f_equal enum_rank).
-      rewrite 2!enum_valK => H2. move: H1.
-      by rewrite H2 eq_refl.
-    move => H0 /existsP [] y /andP [] /andP [] /orP [] H1 H2 H3.
-    simpl.
-    case_eq (i==j).
-      move/eqP => H4. rewrite H4 eq_refl der_Plus der_fold_Plus mem_der_Plus.
-      apply/orP. left.
-      rewrite -mem_der_fold_Plus.
-      apply/orP. right.
-      
-      apply: mem_der_fold_Plus.
-      right.
-      rewrite 2!has_map.
-      apply/hasP.
-      exists a.
-      rewrite mem_filter.
-      simpl.
-      
-      
-      
-      
-      
-      by rewrite eq_refl /= orbT.
-      
-  elim: w k i j => [|a w IHw] k i j.
-    elim: k i j => [|k IHk] i j //.
-    simpl.
-    case_eq (i==j).
-      move/eqP => -> H0 _.
-      by rewrite eq_refl /= orbT.
-    move => H1 H0 /eqP /(f_equal enum_rank).
-    rewrite 2!enum_valK => H2. move: H1.
-    by rewrite H2 eq_refl.
-  move => H0 /=.
-  move /eqP /(f_equal enum_rank). rewrite 2!enum_valK => ->.
-  apply/orP. right.
-  apply: IHk.
-    exact: H0.
-  by rewrite /= eq_refl.
-move => H0.
-rewrite /nfa_lang /=.
-move/existsP => [] y /andP [] /andP [] /orP [] H1 H2 H3.
-  apply: IHw.
-  
-  
-  simpl.
-
-  
-
-Lemma R_correct0' x a y : dfa_step A x a = y ->
-   has_eps
-     (der a
-        (foldr (@Plus char) (Void char)
-           (map (Atom (symbol:=char))
-              (filter
-                 [pred a0 : char |
-                  dfa_step A (enum_val (enum_rank x)) a0 ==
-                  enum_val (enum_rank y)] (enum char))))).
-Proof. move => H0.
-  rewrite der_fold_Plus.
-  apply: has_eps_fold_Plus.
-  right. exists (Eps _).
-  rewrite /= andbT.
-  apply/mapP.
-  exists (Atom a).
-    apply/mapP.
-    exists a.
-      by rewrite mem_filter /= 2!enum_rankK H0 eq_refl andTb mem_enum.
-    by [].
-  by rewrite /= eq_refl.
-Qed.
-   
-
-Lemma R_correct0 x a y: dfa_step A x a = y -> has_eps (der a (R 0 (enum_rank x) (enum_rank y))).
-Proof.
-case_eq (x == y) => /=.
-  move/eqP => ->. rewrite eq_refl => /=.
-  rewrite orbF. exact: R_correct0'.
-move => H0.
-assert (enum_rank x == enum_rank y = false).
-  apply/eqP.
-  move/(f_equal enum_val).
-  rewrite 2!enum_rankK.
-  move => H1. move: H1 H0 => ->. by rewrite eq_refl. 
-rewrite H.
-exact: R_correct0'.
-Qed.
-
-Lemma R_correct1 k x a w y:
-  let x' := dfa_step A x a in
-  let xs := dfa_run' A x' w in
-  all [ pred x | enum_rank x < k] (belast x' xs) ->
-  last x' xs = y ->
-  mem_der (R k (enum_rank x) (enum_rank y)) (a::w).
-Proof.
-elim: w k a x y => [|b w IHw] k a x y.
-  elim: k a x y => [|k IHk] a x y x' xs H0 H1.
-    by apply: R_correct0.
-  simpl in H0,H1.
-  rewrite -H1.
-  rewrite /=. apply/orP. right.
-  move: (IHk _ _ _ H0 H1).
-  by rewrite -H1.
-elim: k w IHw a x y => [|k IHk] w IHw a x y x' xs H0 H1 //.
-move: (IHk _ IHw). clear IHk => IHk.
-simpl R.
-rewrite mem_der_Plus.
-
-
-
-assert ([pred x0 | enum_rank x0 < k.+1] =1 [pred x0 : A | (enum_rank x0 < k) || (k == enum_rank x0) ]).
-  move => x0.
-  rewrite /= leq_eqVlt -{2}(addn1 (enum_rank x0)) -{2}(addn1 k) ltn_add2r.
-  rewrite orbC eq_sym.
-  case_eq (enum_rank x0 < k) => -> //=.
-move: H0.
-rewrite (eq_all H).
-rewrite all_predI.
-
-
-move => x' xs H0 H1.
-simpl.
-elim: k w IHw a x y => [|k IHk] a x y x' xs H0 H1.
-   
-
-  
-elim: k x a w y => [|k IHk] x a w y.
-  elim: w a x y => [|b w IHw] a x y //=.
-  move => _.
-  exact: R_correct0.
-elim: w k IHk a x y => [|b w IHw] k IHk a x y.
-  rewrite /dfa_run' /last.
-  rewrite /belast => _.
-  move => H0.
-  apply/orP. right.
-  exact: (IHk x a [::] y is_true_true H0).
-move => x' xs.
-rewrite [last x' xs]/= [all _ _]/=.
-move/andP => [] H0 H1 H2.  
-
-(* alternative 1 *)
-move: (IHw _ IHk). clear IHw => IHw.
-
-move Eqw': (b::w) => w'.
-rewrite /= mem_der_Plus.
-move Eqk': (Ordinal (n:=#|A|) (m:=minn k #|A|.-1)
-                    (noname (minn k #|A|.-1) #|A| A_has_states
-                       (minn_to_ord k #|A|.-1))) => k'.
-
-(* Decide whether the new run goes over the newly
-   included state. *)
-move: H0. rewrite leq_eqVlt orbC -{1}(addn1 k) -{1}(addn1 (enum_rank x')) ltn_add2r => /orP [].
-  move => H0.
-  apply/orP. right.
-  apply: IHk.
-  
-
-case_eq (x' == enum_val k').
-  move/eqP => H3.
-  rewrite 2!fun_if if_arg.
-  case_eq (has_eps (R k (enum_rank x ) k')) => H4.
-    rewrite mem_der_Plus.
-    rewrite -Eqw'. rewrite (mem_der_Conc _ _ [::b] w).
-    rewrite mem_der_Plus.
-    rewrite (mem_der_Conc _ _ [::b] w).
-    
-    apply/orP. left.
-    rewrite [der b _]/= .
-    
-    assert (has_eps (der a (R k (enum_rank x) k'))).
-      move: (IHk x a [::] (enum_val k') is_true_true H3).
-      by rewrite /= enum_valK.
-    rewrite H 2!mem_der_Plus.
-    apply/orP. left. apply/orP. left.
-    eapply (mem_der_Conc _ _).
-    
-    
-
-
-
-
-
-(* alternative 2 *)
-
-move: H0. rewrite leq_eqVlt => /orP [].
-  move/eqP/(f_equal predn) => H0. simpl in H0. 
-  rewrite /= mem_der_Plus. apply/orP. left.
-  move Eqk': (Ordinal (n:=#|A|) (m:=minn k #|A|.-1)
-                    (noname (minn k #|A|.-1) #|A| A_has_states
-                       (minn_to_ord k #|A|.-1))) => k'.
-  rewrite 2!fun_if if_arg der_Plus mem_der_Plus.
-  case_eq (has_eps (R k (enum_rank x ) k')) => H3.
-    rewrite der_Plus.
-    apply/orP. left.
-    rewrite [der b _]/= .
-
-    assert (x' = enum_val k').
-      rewrite -H0.
-    
-    assert (has_eps (der a (R k (enum_rank x) k'))).
-    move: (IHk x' a [::] (enum_val k') is_true_true).
-    
-        
-
-  
-
-
-End TransitiveClosure.
-
-
-
-Section StateRemoval.
-  
-Variable char: finType.
-Definition word:= misc.word char.
-  
-Record re_nfa : Type :=
-  re_nfaI {
-    re_nfa_state :> finType;
-    re_nfa_s0: re_nfa_state;
-    re_nfa_fin: pred re_nfa_state;
-    re_nfa_re: re_nfa_state -> re_nfa_state -> regular_expression char
-    }.
-
-Variable A: nfa char.
-
-Definition nfa_to_re_nfa: re_nfa :=
-  re_nfaI
-    (option_finType A)
-    (Some (nfa_s0 A))
-    (fun x => if x is Some x then false else true)
-    (fun x y =>
-       if x is Some x then
-         if y is Some y then
-            foldr
-              (@Plus char)
-              (@Void char)
-              (map (@Atom char) (enum [pred a | nfa_step A x a y]))
-         else
-           if nfa_fin A x then
-             (@Eps char)
-           else
-             @Void char
-       else
-         if y is Some y then
-           @Void char
-         else
-           @Eps char
-    )
-    .
-    
-Section Acceptance.
-Variable R: re_nfa.
-
-
-Definition re_nfa_step: R -> word -> pred R :=
-fun x w y => mem_der (re_nfa_re R x y) w.
-
-Lemma size_ind (P: word -> Type):
-  (forall w, (forall w', size w' < size w -> P w') -> P w) ->
-  forall w, P w.
-Proof.
-move => H w.
-move Heqn: (size w) => n.
-assert (size w <= n). by rewrite Heqn.
-clear Heqn.
-elim: n w H0 => [|n IHn] w.
-  rewrite leqn0. move/eqP/size0nil => ->. by apply: H.
-rewrite leq_eqVlt.
-case_eq (size w == n.+1); case_eq (size w < n.+1) => //.
-    move => H1 _ _. by apply: IHn.
-  move => _ /eqP H1 _. apply: H.
-  rewrite H1. exact: IHn.
-move => H1 _ _. by apply: IHn.
-Qed.
-
-Lemma sub0 n: n - 0 = n.
-elim: n => [|n IHn] //.
-Qed.                    
-
-Lemma drop_size_gt0 n (w: word) : size w > 0 -> n > 0 -> size (drop n w) < size w.
-Proof.
-rewrite size_drop.
-move => H.
-rewrite leq_eqVlt => /orP [].
-  move/eqP => H1. move: H. rewrite -H1 subn1 => H.
-  rewrite -(ltn_add2r 1) addn1 prednK -addn1 //.
-move => H1.
-assert (size w -n < size w - 0).
-  apply: ltn_sub2l => //.
-  move: H1.
-  by apply: ltn_trans.
-move: H0.
-by rewrite sub0.
-Qed.
-
-  
-Lemma re_nfa_accept (x: R) (w: word): bool.
-Proof.
-move: w x. apply: size_ind.
-move => [|a w] F x.
-  exact: re_nfa_fin x.
-exact
-(
-  existsb n: 'I_(size (a::w)),
-    existsb y: R,
-      re_nfa_step x (take n.+1 (a::w)) y
-    && F (drop n.+1 (a::w)) (drop_size_gt0 _ (a::w) (ltn0Sn _) (ltn0Sn _)) y
-).
-Defined.
-
-End Acceptance.
-
-Lemma nfa_to_re_nfa_correct1 x w: nfa_accept A x w -> re_nfa_accept (nfa_to_re_nfa) (Some x ) w.
-Proof. 
-elim: w x => [|a w IHw] x /=.
-  move => H0.
-  rewrite /re_nfa_accept /size_ind /=.
-
-    
-                                          
-End StateRemoval.
-
-
-
+    by apply: IHk.
